Fomega/Proof.lean
@@ -5,16 +5,16 @@ import Fomega.Ctx
 namespace Fomega
 
   inductive Conv : Term -> Term -> Prop
-  | ax : Conv ★ ★
+  | ax : Conv (.const K) (.const K)
   | bound x : Conv (.bound K x) (.bound K x)
   | all_congr : Conv A1 A2 -> Conv B1 B2 -> Conv (.all mf A1 B1) (.all mf A2 B2)
   | lam_congr : Conv A1 A2 -> Conv t1 t2 -> Conv (.lam mf A1 t1) (.lam mf A2 t2)
-  | lam_eta1 :
-    Conv (.lam mf A t1) (Term.eta mf A t2) ->
-    Conv (.lam mf A t1) t2
-  | lam_eta2 :
-    Conv (Term.eta mf A t1) (.lam mf A t2) ->
-    Conv t1 (.lam mf A t2)
+  -- | lam_eta1 :
+  --   Conv (.lam mf A t1) (Term.eta mf A t2) ->
+  --   Conv (.lam mf A t1) t2
+  -- | lam_eta2 :
+  --   Conv (Term.eta mf A t1) (.lam mf A t2) ->
+  --   Conv t1 (.lam mf A t2)
   | app_congr : Conv f1 f2 -> Conv a1 a2 -> Conv (.app m f1 a1) (.app m f2 a2)
   | app_beta1 :
     Conv (b β[t]) t2 ->
@@ -32,9 +32,8 @@ namespace Fomega
   inductive Proof : Ctx -> Term -> Term -> Prop
   | ax : Proof Γ ★ □
   | var :
-    A = Γ d@ x ->
-    Proof Γ A (.const K) ->
-    Proof Γ (.bound K x) A
+    -- Proof Γ A (.const K) ->
+    Proof Γ (.bound K x) (Γ d@ x)
   | pi :
     Proof Γ A (.const K) ->
     Proof (A::Γ) B ★ ->
@@ -57,6 +56,17 @@ namespace Fomega
     Proof Γ B (.const K) ->
     A === B ->
     Proof Γ t B
+
+  inductive Wf : Term -> Ctx -> Prop
+  | ax : Wf ★ Γ
+  | var :
+    Proof Γ (Γ d@ x) (.const K) ->
+    Wf (.bound K x) Γ
+  | pi : Wf A Γ -> Wf B (A::Γ) -> Wf (.all mf A B) Γ
+  | lam : Wf A Γ -> Wf B (A::Γ) -> Wf (.lam mf A B) Γ
+  | app : Wf f Γ -> Wf a Γ -> Wf (.app mf f a) Γ
+
 end Fomega
 
 notation:170 Γ:170 " ⊢ " t:170 " : " A:170 => Fomega.Proof Γ t A
+notation:170 t:170 " ⊢ " Γ:170 => Fomega.Wf t Γ
