Fomega/Basic.lean
@@ -1,0 +1,7 @@
+
+import Fomega.Basic.Classification
+import Fomega.Basic.Conv
+import Fomega.Basic.Inversion
+import Fomega.Basic.Strengthen
+import Fomega.Basic.Substitution
+import Fomega.Basic.Weaken
