Fomega/Basic/Classification.lean
@@ -1,0 +1,52 @@
+import Common
+import Fomega.Ctx
+import Fomega.Proof
+import Fomega.PreProof
+import Fomega.Basic.Conv
+import Fomega.Basic.Weaken
+import Fomega.Basic.Substitution
+import Fomega.Basic.Inversion
+
+namespace Fomega.Proof
+
+  theorem proof_classification : t ⊢ Γ -> Γ ⊢ t : A -> A = □ ∨ (∃ K, Γ ⊢ A : .const K) := by
+  intro j1 j2
+  induction j2
+  case ax => apply Or.inl; rfl
+  case var Γ K x =>
+    apply Or.inr; cases j1
+    case _ j => exists K
+  case pi =>
+    apply Or.inr
+    exists .kind; constructor
+  case tpi => apply Or.inl; rfl
+  case lam Γ A B K t h1 _h2 _ih1 _ih2 =>
+    apply Or.inr; exists K
+  case app Γ f A B a B' _h1 h2 h3 ih1 _ih2 =>
+    cases j1
+    case _ j1 j2 =>
+      replace ih1 := ih1 j1
+      cases ih1 <;> simp at *
+      case _ h =>
+        cases h
+        case _ K h =>
+          cases h
+          case _ K q1 q2 =>
+            have h := Proof.beta q2 h2; simp at h
+            apply Or.inr; exists .type
+            subst h3; exact h
+          case _ K q1 q2 =>
+            have h := Proof.beta q2 h2; simp at h
+            apply Or.inr; exists .kind
+            subst h3; exact h
+          case _ T K' q1 q2 q3 =>
+            replace q1 := all_destruct q1 q2
+            replace q1 := beta q1 h2
+            replace q2 := Conv.beta (IsPreProof.from_proof h2) q2
+            apply Or.inr; exists K
+            apply Proof.conv; subst h3; simp at *
+            apply q1; apply q3; apply q2
+  case conv K _h1 h2 _h3 _ih1 _ih2 =>
+    apply Or.inr; exists K
+
+end Fomega.Proof
