Fomega/Basic/Conv.lean
@@ -1,0 +1,166 @@
+
+import Common
+import Fomega.Ctx
+import Fomega.Proof
+import Fomega.PreProof
+
+namespace Fomega.Conv
+
+  theorem refl : IsPreProof A -> A === A := by
+  intro j
+  induction j <;> (constructor <;> simp [*])
+
+  theorem sym :
+    IsPreProof A ->
+    IsPreProof B ->
+    A === B ->
+    B === A
+  := by
+  intro p1 p2 j
+  induction j
+  case ax => constructor
+  case bound => constructor
+  case all_congr ih1 ih2 =>
+    cases p1
+    case _ p11 p12 =>
+      cases p2
+      case _ p21 p22 =>
+        constructor
+        case _ => apply ih1 p11 p21
+        case _ => apply ih2 p12 p22
+  case lam_congr ih1 ih2 =>
+    cases p1
+    case _ p11 p12 =>
+      cases p2
+      case _ p21 p22 =>
+        constructor
+        case _ => apply ih1 p11 p21
+        case _ => apply ih2 p12 p22
+  -- case lam_eta1 ih =>
+  --   apply Conv.lam_eta2; apply ih p1
+  --   unfold Term.eta; simp; constructor
+  --   case _ => cases p1; simp [*]
+  --   case _ =>
+  --     constructor
+  --     case _ => apply IsPreProof.ren p2
+  --     case _ => constructor
+  -- case lam_eta2 ih =>
+  --   apply Conv.lam_eta1; apply ih _ p2
+  --   unfold Term.eta; simp; constructor
+  --   case _ => cases p2; simp [*]
+  --   case _ =>
+  --     constructor
+  --     case _ => apply IsPreProof.ren p1
+  --     case _ => constructor
+  case app_congr ih1 ih2 =>
+    cases p1
+    case _ p11 p12 =>
+      cases p2
+      case _ p21 p22 =>
+        constructor
+        case _ => apply ih1 p11 p21
+        case _ => apply ih2 p12 p22
+  case app_beta1 ih =>
+    cases p1
+    case _ p11 p12 =>
+      cases p11
+      case _ p111 p112 =>
+        apply Conv.app_beta2; apply ih _ p2
+        apply IsPreProof.beta p112 p12
+  case app_beta2 ih =>
+    cases p2
+    case _ p11 p12 =>
+      cases p11
+      case _ p111 p112 =>
+        apply Conv.app_beta1; apply ih p1
+        apply IsPreProof.beta p112 p12
+
+  theorem rename : A === B -> ([r#r]A) === ([r#r]B) := by
+  intro j; induction j generalizing r <;> simp
+  case ax => constructor
+  case bound K x => constructor
+  case all_congr A1 A2 B1 B2 _j1 _j2 ih1 ih2 =>
+    constructor; apply ih1
+    replace ih2 := @ih2 (Term.Ren.lift r); simp at ih2
+    apply ih2
+  case lam_congr A1 A2 t1 t2 _j1 _j2 ih1 ih2 =>
+    constructor; apply ih1
+    replace ih2 := @ih2 (Term.Ren.lift r); simp at ih2
+    apply ih2
+  -- case lam_eta1 A' t1 t2 _j ih =>
+  --   apply Conv.lam_eta1; simp at *; apply ih
+  -- case lam_eta2 A' t1 t2 _j ih =>
+  --   apply Conv.lam_eta2; simp at *; apply ih
+  case app_congr f1 f2 a1 a2 m _j1 _j2 ih1 ih2 =>
+    constructor; apply ih1; apply ih2
+  case app_beta1 t b t2 A' _j ih =>
+    apply Conv.app_beta1; simp at *; apply ih
+  case app_beta2 t b t2 A' _j ih =>
+    apply Conv.app_beta2; simp at *; apply ih
+
+  theorem subst : (∀ n s, σ n = .replace s -> IsPreProof s) -> A === B -> ([σ]A) === ([σ]B) := by
+  intro h j
+  induction j generalizing σ <;> simp
+  case ax => constructor
+  case bound _ x =>
+    generalize ydef : σ x = y at *
+    cases y <;> simp at *
+    case _ => constructor
+    case _ => apply refl; apply h x _ ydef
+  case all_congr _j1 _j2 ih1 ih2 =>
+    constructor; apply ih1 h
+    replace ih2 := @ih2 (^σ) (IsPreProof.lift h); simp at ih2; exact ih2
+  case lam_congr _j1 _j2 ih1 ih2 =>
+    constructor; apply ih1 h
+    replace ih2 := @ih2 (^σ) (IsPreProof.lift h); simp at ih2; exact ih2
+  -- case lam_eta1 _j ih =>
+  --   constructor; simp at ih; unfold Term.eta; simp
+  --   apply ih h
+  -- case lam_eta2 _j ih =>
+  --   constructor; simp at ih; unfold Term.eta; simp
+  --   apply ih h
+  case app_congr _j1 _j2 ih1 ih2 =>
+    constructor; apply ih1 h; apply ih2 h
+  case app_beta1 _j ih =>
+    simp at *; constructor; simp; apply ih h
+  case app_beta2 _j ih =>
+    simp at *; constructor; simp; apply ih h
+
+  theorem beta : IsPreProof t -> A === B -> (A β[t]) === (B β[t]) := by
+  intro p h; simp; apply subst
+  case _ =>
+    intro n t' h2
+    cases n <;> simp at h2
+    subst h2; exact p
+  case _ => exact h
+
+  theorem trans2 :
+    IsPreProof A -> Γ ⊢ B : T -> IsPreProof C ->
+    A === B -> B === C -> A === C
+  := by
+  intro p1 j p3 h1 h2
+  induction j generalizing A C
+  case ax => sorry
+  case var => sorry
+  case pi => sorry
+  case tpi => sorry
+  case lam => sorry
+  case app ih1 ih2 => sorry
+  case conv h ih1 ih2 => apply ih1 p1 p3 h1 h2
+
+  theorem trans :
+    IsPreProof A -> IsPreProof B -> IsPreProof C ->
+    A === B -> B === C -> A === C
+  := by
+  intro p1 p2 p3 h1 h2
+  induction h1 generalizing C
+  case _ => simp [*]
+  case _ => simp [*]
+  case all_congr => sorry
+  case lam_congr => sorry
+  case app_congr => sorry
+  case app_beta1 => sorry
+  case app_beta2 => sorry
+
+
+end Fomega.Conv
