Fomega/Basic/Inversion.lean
@@ -1,0 +1,40 @@
+
+import Common
+import Fomega.Ctx
+import Fomega.Proof
+import Fomega.PreProof
+import Fomega.Basic.Conv
+import Fomega.Basic.Weaken
+
+namespace Fomega.Proof
+
+  theorem all_destruct :
+    Γ ⊢ .all mf A B : T ->
+    T === .const K ->
+    (A::Γ) ⊢ B : T
+  := by
+  intro j hc
+  generalize tdef : Term.all mf A B = t at *
+  induction j generalizing A B
+  case ax => simp at tdef
+  case var => simp at tdef
+  case pi => sorry
+  case tpi => sorry
+  case lam => simp at tdef
+  case app => simp at tdef
+  case conv Γ t' A' B' K' h1 h2 h3 ih1 ih2 =>
+    cases t' <;> simp at tdef
+    case _ m r1 r2 =>
+      cases tdef
+      case _ e1 h' =>
+        cases h'
+        case _ e2 e3 =>
+          subst e1; subst e2; subst e3
+          have ih3 := @ih1 A B sorry rfl
+          apply Proof.conv; exact ih3
+          sorry
+          exact h3
+          exact K
+
+
+end Fomega.Proof
