Fomega/Basic/Strengthen.lean
@@ -1,0 +1,147 @@
+import Common
+import Fomega.Ctx
+import Fomega.Proof
+import Fomega.PreProof
+import Fomega.Basic.Conv
+
+namespace Fomega.Proof
+
+  abbrev Iℓ (ℓ : Nat) : Subst Term
+  | 0 => .rename ℓ
+  | n + 1 => .rename (n + 1)
+
+  abbrev repIℓ n ℓ := ^{n}(Iℓ ℓ)
+
+  abbrev Pℓ (ℓ : Nat) : Subst Term
+  | 0 => .rename ℓ
+  | n + 1 => .rename n
+
+  abbrev repPℓ n ℓ := ^{n}(Pℓ ℓ)
+
+  @[simp]
+  theorem Iℓ_after_S : (Iℓ ℓ) ⊙ S = S := by
+  funext
+  case _ x =>
+    cases x <;> simp at *
+    <;> unfold Term.Subst.compose at *
+    <;> simp at *
+
+  theorem repIℓ_eq ℓ : n = x -> (repIℓ n ℓ) x = .rename (ℓ + x) := by
+  intro h
+  induction n generalizing x <;> simp
+  case _ => subst h; simp
+  case _ n ih =>
+    simp at ih; unfold repIℓ at ih
+    subst h; simp; unfold Term.Subst.compose; simp
+    rw [ih]; simp; omega
+
+  theorem repIℓ_neq ℓ : n ≠ x -> (repIℓ n ℓ) x = .rename x := by
+  intro h
+  induction n generalizing x <;> simp
+  case _ => unfold Iℓ; cases x <;> simp at *
+  case _ n ih =>
+    cases x <;> simp
+    case _ x =>
+      have nh : n ≠ x := by omega
+      unfold Term.Subst.compose
+      have ih' := ih nh
+      simp; unfold repIℓ at ih'; rw [ih']
+
+  @[simp]
+  theorem Pℓ_after_S : (Pℓ ℓ) ⊙ S = I := by
+  funext
+  case _ x =>
+    cases x <;> simp at *
+    <;> unfold Term.Subst.compose at *
+    <;> simp at *
+
+  theorem repPℓ_lt ℓ : n < x -> (repPℓ n ℓ) x = .rename (x - 1) := by
+  intro h
+  induction n generalizing x <;> simp
+  case _ =>
+    cases x <;> simp at *
+  case _ n ih =>
+    cases x <;> simp
+    case _ x =>
+      unfold Term.Subst.compose; simp
+      have nh : n < x := by omega
+      have ih' := ih nh; simp at ih'
+      unfold repPℓ at ih'; rw [ih']; simp
+      cases x <;> simp at *
+
+  theorem repPℓ_eq ℓ : n = x -> (repPℓ n ℓ) x = .rename (ℓ + x) := by
+  intro h
+  induction n generalizing x <;> simp
+  case _ => subst h; simp
+  case _ n ih =>
+    simp at ih; unfold repPℓ at ih
+    subst h; simp; unfold Term.Subst.compose; simp
+    rw [ih]; simp; omega
+
+  theorem repPℓ_ge ℓ : n > x -> (repPℓ n ℓ) x = .rename x  := by
+  intro h
+  induction n generalizing x <;> simp
+  case _ => omega
+  case _ n ih =>
+    cases x <;> simp
+    case _ x =>
+      have nh : n > x := by omega
+      unfold Term.Subst.compose
+      have ih' := ih nh
+      simp; unfold repPℓ at ih'; rw [ih']
+
+
+  -- theorem strengthen_nth_lift_ge n :
+  --   (∀ x, x ≥ n → Γ d@ (x + 1) = [^{n}S]Δ d@ x) ->
+  --   ∀ x, x ≥ n + 1 → (U :: Γ)d@(x + 1) = [^{n + 1}S](V :: Δ)d@x
+  -- := by
+  -- intro h1 x h2
+  -- cases x <;> simp
+  -- case _ => omega
+  -- case _ x =>
+  --   replace h2 : x ≥ n := by omega
+  --   replace h1 := h1 x h2
+  --   rw [h1]; simp
+
+  -- theorem strengthen_nth_lift_ge2 A n :
+  --   (∀ x, x ≥ n -> [^{n}P]Γ d@ (x + 1) = Δ d@ x) ->
+  --   ∀ x, x ≥ n + 1 → [^{n + 1}P](A :: Γ) d@ (x + 1) = ([^{n}P]A :: Δ)d@x
+  -- := by sorry
+
+  -- theorem strengthen_nth_lift_lt n :
+  --   [^{n}S]V = U ->
+  --   (∀ x, x < n -> Γ d@ x = [^{n}S]Δ d@ x) ->
+  --   ∀ x, x < n + 1 → (U :: Γ)d@x = [^{n + 1}S](V :: Δ)d@x
+  -- := by
+  -- intro h0 h1 x h2
+  -- cases x <;> simp
+  -- case _ => rw [<-Term.subst_apply_compose_commute, h0]
+  -- case _ x =>
+  --   replace h2 : x < n := by omega
+  --   rw [h1 x h2]; simp
+
+  -- theorem strengthen_nth_lift_lt2 A n :
+  --   (∀ x, x < n -> [^{n}P]Γ d@ x = Δ d@ x) ->
+  --   ∀ x, x < n + 1 → [^{n + 1}P](A :: Γ)d@x = ([^{n}P]A :: Δ)d@x
+  -- := by sorry
+
+  -- theorem strengthen_nth2 n  :
+  --   Γ ⊢ t : T ->
+  --   [repIℓ n Γ.length]t = t ->
+  --   IsPreKind T ->
+  --   (∀ x, x < n -> [repPℓ n Γ.length]Γ d@ x = Δ d@ x) ->
+  --   (∀ x, x + 1 ≥ n -> [repPℓ n Γ.length]Γ d@ (x + 1) = Δ d@ x) ->
+  --   Δ ⊢ ([repPℓ n Γ.length]t) : T
+  -- := by
+
+  -- theorem strengthen : (A :: Δ) ⊢ ([S]t) : .const K -> Δ ⊢ t : .const K := by
+  -- intro j
+  -- have lem := @strengthen_nth2 (A::Δ) _ _ Δ 0 j
+  -- simp at lem; apply lem
+
+  -- theorem strengthen : (A :: Δ) ⊢ ([S]t) : ([S]T) -> Δ ⊢ t : T := by
+  -- intro j
+  -- apply strengthen_nth 0 j
+  -- case _ => intro x nh; omega
+  -- case _ => intro x _; simp
+end Fomega.Proof
