Fomega/Basic/Substitution.lean
@@ -1,0 +1,98 @@
+
+import Common
+import Fomega.Ctx
+import Fomega.Proof
+import Fomega.PreProof
+import Fomega.Basic.Conv
+import Fomega.Basic.Weaken
+
+namespace Fomega.Proof
+
+  theorem lift_subst_rename :
+    (∀ n y, σ n = .rename y -> [σ](Γ d@ n) = Δ d@ y) ->
+    (∀ n y, ^σ n = .rename y -> [^σ]((A :: Γ) d@ n) = ([σ]A :: Δ) d@ y)
+  := by
+  intro h1 n y h2
+  cases n
+  case _ => simp at *; subst h2; simp
+  case _ n =>
+    simp at *; unfold Term.Subst.compose at h2; simp at h2
+    generalize ydef : σ n = y at *
+    cases y <;> simp at h2
+    case _ z =>
+      subst h2; simp
+      replace h1 := h1 n z ydef
+      rw [<-Term.subst_apply_compose_commute, h1]
+
+  theorem lift_subst_replace :
+    (∀ n t, σ n = .replace t -> Δ ⊢ t : ([σ]Γ d@ n)) ->
+    (∀ n t, ^σ n = .replace t -> ([σ]A :: Δ) ⊢ t : ([^σ](A :: Γ) d@ n))
+  := by
+  intro h1 n t h2
+  cases n <;> simp at *
+  case _ n =>
+    unfold Term.Subst.compose at h2; simp at h2
+    generalize ydef : σ n = y at *
+    cases y <;> simp at h2
+    case _ t' =>
+      replace h1 := h1 n t' ydef
+      subst h2
+      rw [<-Term.subst_apply_compose_commute]
+      apply weaken; exact h1
+
+  theorem subst :
+    (∀ n t, σ n = .replace t -> IsPreProof t) ->
+    (∀ n y, σ n = .rename y -> [σ](Γ d@ n) = Δ d@ y) ->
+    (∀ n t, σ n = .replace t -> Δ ⊢ t : ([σ]Γ d@ n)) ->
+    Γ ⊢ t : A -> Δ ⊢ ([σ]t) : ([σ]A)
+  := by
+  intro h1 h2 h3 j
+  induction j generalizing Δ σ
+  case _ => constructor
+  case var Γ K x =>
+    simp; generalize ydef : σ x = y at *
+    cases y <;> simp
+    case _ y => rw [h2 x y ydef]; constructor
+    case _ t' => apply h3 x t' ydef
+  case pi Γ' A' K B _j1 _j2 ih1 ih2 =>
+    simp; constructor; apply ih1 h1 h2 h3
+    replace ih2 := @ih2 (^σ) ([σ]A' :: Δ) (IsPreProof.lift h1) (lift_subst_rename h2) (lift_subst_replace h3)
+    simp at ih2; exact ih2
+  case tpi Γ' A' B _j1 _j2 ih1 ih2 =>
+    simp; constructor; apply ih1 h1 h2 h3
+    replace ih2 := @ih2 (^σ) ([σ]A' :: Δ) (IsPreProof.lift h1) (lift_subst_rename h2)  (lift_subst_replace h3)
+    simp at ih2; exact ih2
+  case lam Γ' A' B K t' _j1 _j2 ih1 ih2 =>
+    simp; constructor; simp at *; apply ih1 h1 h2 h3
+    replace ih2 := @ih2 (^σ) ([σ]A' :: Δ) (IsPreProof.lift h1) (lift_subst_rename h2)  (lift_subst_replace h3)
+    simp at ih2; exact ih2
+  case app Γ' f A' B a B' _j1 _j2 j3 ih1 ih2 =>
+    simp; constructor; apply ih1 h1 h2 h3; apply ih2 h1 h2 h3
+    simp at *; subst j3; simp
+  case conv Γ' t' A' B K _j1 _j2 j3 ih1 ih2 =>
+    constructor; apply ih1 h1 h2 h3; apply ih2 h1 h2 h3
+    apply Conv.subst
+    case _ =>
+      intro n s eq
+      apply h1 n s eq
+    case _ => exact j3
+
+  theorem beta : (A::Γ) ⊢ b : B -> Γ ⊢ t : A -> Γ ⊢ (b β[t]) : (B β[t]) := by
+  simp; intro j1 j2
+  apply @subst _ (A::Γ)
+  case _ =>
+    intro n s eq
+    cases n <;> simp at *
+    subst eq; apply IsPreProof.from_proof j2
+  case _ =>
+    intro n y h
+    cases n <;> simp at h
+    case _ n =>
+      subst h; simp
+  case _ =>
+    intro n t' h
+    cases n <;> simp at h
+    case _ => subst h; simp; exact j2
+  case _ => exact j1
+
+end Fomega.Proof
