Fomega/Basic/Weaken.lean
@@ -1,0 +1,60 @@
+
+import Common
+import Fomega.Ctx
+import Fomega.Proof
+import Fomega.PreProof
+import Fomega.Basic.Conv
+
+namespace Fomega.Proof
+
+  theorem rename_lift r A :
+    (∀ x, [r#r](Γ d@ x) = Δ d@ (r x)) ->
+    ∀ x, [r#(Term.Ren.lift r)]((A::Γ) d@ x) = ([r#r]A::Δ) d@ (Term.Ren.lift r x)
+  := by
+  intro h x; simp
+  cases x <;> simp at *
+  case _ x => rw [<-h x]; simp
+
+  theorem rename (r : Ren) : Γ ⊢ t : A ->
+    (∀ x, [r#r](Γ d@ x) = Δ d@ (r x)) ->
+    Δ ⊢ ([r#r]t) : ([r#r]A)
+  := by
+  intro j h
+  induction j generalizing Δ r
+  case ax => constructor
+  case var Γ K x => simp; rw [h x]; constructor
+  case pi Γ' A' K B _j1 _j2 ih1 ih2 =>
+    simp; constructor
+    case _ => apply ih1 r h
+    case _ =>
+      replace ih2 := @ih2 ([r#r]A' :: Δ) (Term.Ren.lift r) (rename_lift r A' h)
+      simp at ih2; exact ih2
+  case tpi Γ' A' B _j1 _j2 ih1 ih2 =>
+    simp; constructor
+    case _ => apply ih1 r h
+    case _ =>
+      replace ih2 := @ih2 ([r#r]A' :: Δ) (Term.Ren.lift r) (rename_lift r A' h)
+      simp at ih2; exact ih2
+  case lam Γ' A' B K t _j1 _j2 ih1 ih2 =>
+    simp; constructor
+    case _ => simp at ih1; apply ih1 r h
+    case _ =>
+      replace ih2 := @ih2 ([r#r]A' :: Δ) (Term.Ren.lift r) (rename_lift r A' h)
+      simp at ih2; exact ih2
+  case app Γ' f A' B a B' _j1 _j2 j3 ih1 ih2 =>
+    simp; constructor
+    case _ => apply ih1 r h
+    case _ => apply ih2 r h
+    case _ => subst j3; simp
+  case conv Γ' t A' B K _j1 _j2 j3 ih1 ih2 =>
+    constructor
+    case _ => apply ih1 r h
+    case _ => apply ih2 r h
+    case _ => apply Conv.rename; apply j3
+
+  theorem weaken B : Γ ⊢ t : A -> (B::Γ) ⊢ ([S]t) : ([S]A) := by
+  intro j; apply rename; exact j
+  case _ => intro x; simp; rw [Term.S_to_rS]; unfold rS; simp
+
+
+namespace Fomega.Proof
